

Integration by Substitution

Q. Evaluate.

i) $\int \sin 4t \, dt$

ii) $\int \frac{\cos 2t}{\sin^3 2t} \, dt$

iii) $\int 4x^3 (\underbrace{x^4 - 1}_u) \, dx$

iv) $\int x^2 \sqrt{\underbrace{4 + x^3}_u} \, dx$

v) $\int \frac{1}{\sqrt{x} (\underbrace{1 + \sqrt{x}}_u)^2} \, dx$

vi) $\int \frac{x}{\sqrt{4 - x^2}} \, dx$

xvii) $\int \sec^2 x \tan x \, dx$

xviii) $\int \tan^3 x \sec^2 x \, dx$

(xix) $\int \sqrt{1 + \sqrt{x}} \, dx$

$\int \left(\frac{1}{x^2} + \frac{5}{x^5} \right) dx$
 $= \int (x^{-2} + 5x^{-5}) \, dx$

vii) $\int \frac{3t}{(t^2 + 1)^2} \, dt$

viii) $\int (x^2 - 3)(x^3 + 2) \, dx$
 open bracket
 apply substitution

ix) $\int \frac{x^3 + 5}{x^5} \, dx$

x) $\int 3x^2 \cos(x^3) \, dx$

xi) $\int x \cos x^2 \, dx$

xii) $\int \sqrt{x} \cos(3\sqrt[3]{x}) \, dx$

like us $\int \sin(7x + 5) \, dx$

xiii) $\int x(x - 3)^5 \, dx$

xiv) $\int \sin^3 x \cos x \, dx$

xv) $\int x \sec^2 x^2 \, dx$

xvi) $\int \sec 2x \tan 2x \, dx$
 like us

$$13) \int \frac{\sin 4t}{u} dt$$

$$\text{let } u = 4t$$

$$\frac{du}{dt} = 4,$$

$$du = 4 dt$$

$$\frac{du}{4} = dt$$

$$\begin{aligned} \int \sin 4t dt &= \int \sin u \frac{du}{4} = \int \frac{1}{4} \sin u du \\ &= \frac{1}{4} \int \sin u du \\ &= -\frac{1}{4} \cos u + C \\ &= -\frac{1}{4} \cos 4t + C \end{aligned}$$

$$xvi) \int \cot 5x \csc 5x dx$$

$$\text{let } u = 5x, \quad du = 5 dx, \quad \frac{du}{5} = dx$$

$$= \int \cot u \csc u \frac{du}{5} = \frac{1}{5} \int \cot u \csc u du$$

$$= -\frac{1}{5} \csc u + C = -\frac{1}{5} \csc(5x) + C$$

$$xi) \int x \cos x^2 dx$$

$$\text{Let } u = x^2$$

$$\frac{du}{dx} = 2x, \quad \frac{du}{2x} = dx$$

$$du = 2x dx$$

$$\int x \cos x^2 dx = \int \cancel{x} \cos u \frac{du}{\cancel{2x}} = \int \frac{1}{2} \cos u du$$

$$= \frac{1}{2} \int \cos u du = \frac{1}{2} \sin u + C$$

$$= \frac{1}{2} \sin x^2 + C$$

→ $u = x^2, du = 2x dx; \frac{du}{2} = x dx$

$$\int x \cos x^2 dx = \int \cos u \frac{du}{2} = \frac{1}{2} \int \cos u du$$

$$= \frac{1}{2} \sin u + C = \frac{1}{2} \sin x^2 + C$$

$$\int \sqrt[3]{x} \cos(3\sqrt[3]{x}) dx$$

let $u = 3\sqrt[3]{x} = 3(x^{1/3})$

$$\frac{du}{dx} = 3 \cdot \frac{1}{3} x^{1/3-1} = x^{-2/3} = (x^{-1/3})^2$$

$$= \left(\frac{1}{x^{1/3}} \right)^2$$

$$= \left(\frac{1}{\sqrt[3]{x}} \right)^2$$

$$\frac{du}{dx} = \frac{1}{(\sqrt[3]{x})^2} \quad \cdot \quad du = \frac{1}{(\sqrt[3]{x})^2} dx$$

$$(\sqrt[3]{x})^2 du = dx$$

$$\int \sqrt[3]{x} \cos(\sqrt[3]{x}) dx = \int \sqrt[3]{x} \cos u (\sqrt[3]{x})^2 du$$

$$a^2 \cdot a^1 = a^{1+2} = a^3$$

$$= \int (\sqrt[3]{x})^3 \cos u du$$

$$u = \sqrt[3]{x}$$

$$\frac{u}{\frac{1}{3}} = \sqrt[3]{x}$$

$$= \left(\frac{u}{\frac{1}{3}}\right)^3 = (\sqrt[3]{x})^3$$

$$\int \frac{u^3}{27} \cos u du$$

$$= \frac{1}{27} \int u^3 \cos u du$$

Requires
integration by
parts.

$$1) \int \frac{\cos 2t}{\sin^3 2t} dt = \int \frac{\cos 2t}{[\sin 2t]^3} dt$$

$$\text{let } u = \sin 2t$$

$$du = 2 \cos 2t dt$$

$$\text{Trig } u \Rightarrow u' \text{ Trig } u$$

$$\frac{du}{2} = \cos 2t dt$$

$$\int \frac{du}{2 \cos 2t} \cdot \frac{\cos 2t}{(\sin 2t)^3} = \int \frac{1}{u^3} \cdot \frac{du}{2} = \frac{1}{2} \int \frac{1}{u^3} du$$

$$= \frac{1}{2} \int u^{-3} du = \frac{1}{2} \frac{u^{-3+1}}{-3+1} + C$$

$$\begin{aligned}
 &= \frac{1}{2} \cdot \frac{\bar{U}^2}{-2} + C = -\frac{1}{4} \frac{1}{U^2} + C \\
 &= -\frac{1}{4} \cdot \frac{1}{(\sin 2t)^2} + C \\
 &= -\frac{1}{4 \sin^2(2t)} + C
 \end{aligned}$$

$$\int \sec^2 x \tan x \, dx$$

$$dv = \sec^2 x \, dx$$

$$u = \tan x \quad \frac{du}{dx} = \sec^2 x \quad du = \sec^2 x \, dx$$

$$\begin{aligned}
 \int \underbrace{\sec^2 x}_{du} \underbrace{\tan x}_u \, dx &= \int \underline{u \, du} = \frac{u^2}{2} + C \\
 &= \frac{\tan^2 x}{2} + C
 \end{aligned}$$

$$\int \sec^2 x \tan x \, dx = \int \sec x \sec x \tan x \, dx$$

$$\text{let } u = \sec x$$

$$du = \sec x \tan x \, dx$$

$$\int u \, du = \frac{u^2}{2} + c$$

$$= \frac{\sec^2 x}{2} + c$$

xviii) $\int \tan^3 x \sec^2 x \, dx$ xiv) $\int \sin^3 x \cos x \, dx$

$$\int \tan^3 x \underbrace{\sec^2 x \, dx}_{du}$$

$$u = \tan x$$

$$du = \sec^2 x \, dx$$

$$du = \sec x \tan x \, dx$$

$$u = \sec x$$

Let $u = \tan x$

$$du = \sec^2 x \, dx$$

$$= \int u^3 \, du = \frac{u^4}{4} + c = \frac{\tan^4 x}{4} + c$$

$$\int \sin^3 x \underbrace{\cos x \, dx}_{du}$$

$$u = \sin x$$

$$du = \cos x \, dx$$

$$u = \cos x$$

$$du = -\sin x \, dx$$

Let $u = \sin x$ $du = \cos x \, dx$

$$\int u^3 du = \frac{u^4}{4} + C = \frac{\sin^4 x}{4} + C$$

$$\int \frac{3t}{(t^2+1)^2} dt$$

$$\text{let } u = t^2 + 1$$

$$du = 2t dt$$

$$\frac{du}{2} = t dt$$

$$\int \frac{3 \cdot \frac{du}{2}}{u^2} = \int \frac{3}{2} \frac{du}{u^2} = \frac{3}{2} \int u^{-2} du$$

$$= \frac{3}{2} \frac{u^{-2+1}}{-2+1} + C$$

$$= \frac{3}{2} \frac{u^{-1}}{-1} + C$$

$$= \frac{3}{2} \frac{1}{-1u} + C$$

$$= -\frac{3}{2(t^2+1)} + C$$

$$\int \frac{x}{\sqrt{4-x^2}} dx$$

$$\text{let } u = 4 - x^2$$

$$\frac{du}{-2x} = dx$$

$$du = -2x dx$$

$$\frac{du}{-2} = x dx$$

$$\int \frac{\cancel{x}}{\sqrt{4-x^2}} \frac{du}{\cancel{-2x}}$$

$$= \int \frac{\frac{du}{-2}}{\sqrt{u}} = \int -\frac{1}{2} \frac{du}{u^{1/2}} = -\frac{1}{2} \int u^{-1/2} du$$

$$= -\frac{1}{2} \frac{u^{-1/2+1}}{-1/2+1} + C$$

$$= -\frac{1}{2} \frac{u^{1/2}}{1/2} + C = -\frac{1}{2} \times 2 \sqrt{u} + C$$

$$= -\sqrt{4-x^2} + C$$

$$\int \frac{1}{u} du = \ln|u| + C = \int \frac{\cos x}{\sin x} dx$$

$$\int e^u du = e^u + C \quad \int x e^{x^2} dx$$

